updated notations, bundle representation, work on thm 3.3

strandspace.v
@@ -21,6 +21,9 @@ Require Import Finite_sets_facts Finite_sets Relation_Definitions.
 Require Import Relation_Operators strictorder util.
 Require Import CoLoRRelDec CoLoRRelSub.
 
+Definition FiniteSet {X:Type} (E:Ensemble X) : Prop :=
+Finite X E.
+
 (* atomic messages *)
 Variable Text : Set.
 Variable eq_text_dec : forall (x y:Text), {x = y} + {x <> y}.
@@ -56,7 +59,7 @@ Hint Constructors Msg.
 Notation "(! x )" := (msg_text x). 
 Notation "(# k )" := (msg_key k).
 Notation "x * y" := (msg_join x y) (at level 40, left associativity). 
-Notation "[ m ]^( k ) " := (msg_encr k m).
+Notation "[ m ]^| k | " := (msg_encr k m).
 
 
 Definition eq_msg_dec : forall x y : Msg,  
@@ -75,21 +78,23 @@ Inductive Subterm : Msg -> Msg -> Prop :=
 | st_join_r : forall st l r, 
                Subterm st r -> Subterm st (l*r)
 | st_encr : forall st t k, 
-               Subterm st t -> Subterm st ([t]^(k)).
+               Subterm st t -> Subterm st ([t]^|k|).
 (* [REF 1] Section 2.1 pg 6 and Definition 2.11 *)
 Hint Constructors Subterm.
 
+Notation "a <st b" := (Subterm a b) (at level 30).
+
 (* signed message, + (tx) or - (rx) *)
 Inductive SMsg : Type := 
-| tx : Msg -> SMsg
-| rx : Msg -> SMsg.
+| msg_tx : Msg -> SMsg
+| msg_rx : Msg -> SMsg.
 (* [REF 1] Definition 2.1 pg 6 
    They are defined as a pair, w/ the first member being in {+, -} 
    and the second a signed message. *)
 Hint Constructors SMsg.
 
-Notation "(+ x )" := (tx x).
-Notation "(- x )" := (rx x).
+Notation "(+ x )" := (msg_tx x).
+Notation "(- x )" := (msg_rx x).
 
 Definition eq_smsg_dec : forall x y : SMsg,  
   {x = y} + {x <> y}.
@@ -147,7 +152,7 @@ Definition EdgeSet := Ensemble Edge.
 
 
 (* index of a node *)
-Definition Node_index (n:Node) : nat :=
+Definition index (n:Node) : nat :=
   match n with
     | exist npair _ 
       => snd npair
@@ -155,18 +160,14 @@ Definition Node_index (n:Node) : nat :=
 (* [REF 1] Definition 2.3.2 pg 6
    "If n = <s,i> then index(n) = i." *)
 
-Notation "index( x )" := (Node_index x).
-
 (* strand of a node *)
-Definition Node_strand (n:Node) : Strand :=
+Definition strand (n:Node) : Strand :=
   match n with
     | exist npair _ 
       => fst npair
   end.
 (* [REF 1] Definition 2.3.2 pg 6
    "If n = <s,i> then ... strand(n) = s." *)
-
-Notation "strand( x )" := (Node_strand x).
 
 (* signed message of a node *)
 Fixpoint Node_smsg_option (n:Node) : (option SMsg) :=
@@ -213,31 +214,27 @@ Proof.
 Qed.
 
 (* signed message of a node *)
-Definition Node_smsg (n:Node) : SMsg :=
+Definition smsg (n:Node) : SMsg :=
   match node_smsg_valid n with
     | exist m _ => m
   end.
 
-Notation "smsg( x )" := (Node_smsg x).
-
 (* unsigned message of a node *)
-Definition Node_msg (n:Node) : Msg :=
-  match Node_smsg n with
-    | tx t => t
-    | rx t => t
+Definition msg (n:Node) : Msg :=
+  match smsg n with
+    | (+t) => t
+    | (-t) => t
   end. 
 (* [REF 1] Definition 2.3.2 pg 6
    "Define uns_term(n) to be the unsigned part of the ith signed term 
     of the trace of s." *)
-
-Notation "msg( x )" := (Node_msg x).
 
 Lemma node_smsg_msg_tx : forall n t,
 smsg(n) = (+ t) ->
 msg(n) = t.
 Proof.
   intros n t nsmsg.
-  unfold Node_msg. rewrite nsmsg. reflexivity. 
+  unfold msg. rewrite nsmsg. reflexivity. 
 Qed.
 
 Lemma node_smsg_msg_rx : forall n t,
@@ -245,14 +242,14 @@ smsg(n) = (- t) ->
 msg(n) = t.
 Proof.
   intros n t nsmsg.
-  unfold Node_msg. rewrite nsmsg. reflexivity. 
+  unfold msg. rewrite nsmsg. reflexivity. 
 Qed.
 
 Definition is_tx (n:Node) : Prop :=
-exists t, Node_smsg n = (+ t).
+exists t, smsg n = (+ t).
 
 Definition is_rx (n:Node) : Prop :=
-exists t, Node_smsg n = (- t).
+exists t, smsg n = (- t).
 
 Definition eq_node_dec : forall x y : Node,
  {x = y} + {x <> y}.
@@ -310,14 +307,14 @@ Hint Constructors Comm.
   may send or receive a message but not both at the 
   same time". *)
 
-Notation "a --> b" := (Comm a b) (at level 30, right associativity). 
+Notation "a --> b" := (Comm a b) (at level 0, right associativity). 
 
 Lemma comm_dec : forall x y,
 {x --> y} + {~ x --> y}.
 Proof.
   intros x y.
-  remember (Node_smsg x) as xsmsg. remember (Node_smsg y) as ysmsg.
-  remember (Node_strand x) as xstrand. remember (Node_strand y) as ystrand.
+  remember (smsg x) as xsmsg. remember (smsg y) as ysmsg.
+  remember (strand x) as xstrand. remember (strand y) as ystrand.
   destruct xsmsg.
   Case "x (tx m)".
     destruct ysmsg.
@@ -386,14 +383,14 @@ Inductive Successor : relation Node :=
    "When n1= <s,i> and n2=<s,i+1> are members of N (set of node), there is
     an edge n1 => n2." *)
 
-Notation "a ==> b" := (Successor a b)  (at level 30, right associativity). 
+Notation "a ==> b" := (Successor a b)  (at level 0, right associativity). 
 
 Lemma succ_dec : forall x y,
 {x ==> y} + {~ x ==> y}.
 Proof.
   intros x y.
-  remember (Node_index x) as xi. remember (Node_index y) as yi.
-  remember (Node_strand x) as xstrand. remember (Node_strand y) as ystrand.
+  remember (index x) as xi. remember (index y) as yi.
+  remember (strand x) as xstrand. remember (strand y) as ystrand.
   destruct (eq_strand_dec xstrand ystrand) as [seq | sneq].
   Case "strands eq".
     destruct (eq_nat_dec yi (S xi)) as [succi | wrongi].
@@ -431,7 +428,7 @@ clos_trans Successor.
     the same strand." *)
 Hint Constructors clos_trans.
 
-Notation "a ==>+ b" := (StrandPath a b)  (at level 30, right associativity). 
+Notation "a ==>+ b" := (StrandPath a b)  (at level 0, right associativity). 
 
 Lemma spath_imp_eq_strand : forall x y,
 x ==>+ y -> strand(x) = strand(y).
@@ -533,7 +530,7 @@ Hint Resolve ssedge_antisymmetry.
 Definition SSPath : relation Node := 
 clos_trans SSEdge.
 
-Notation "a << b" := (SSPath a b) (at level 30, right associativity). 
+Notation "a << b" := (SSPath a b) (at level 0, right associativity). 
 
 Theorem spath_imp_sspath : forall i j,
 i ==>+ j -> i << j.
@@ -558,7 +555,7 @@ Definition SSPathEq : relation Node :=
 clos_refl_trans SSEdge.
 Hint Constructors clos_refl_trans.
 
-Notation "a <<* b" := (SSPathEq a b) (at level 30, right associativity). 
+Notation "a <<* b" := (SSPathEq a b) (at level 0, right associativity). 
 
 Theorem sspatheq_opts: forall n m,
 n <<* m -> n << m \/ n = m.
@@ -596,55 +593,49 @@ Inductive InPair {X:Type} (E:Ensemble (X*X)) (x:X): Prop :=
           -> InPair E x.
 Hint Constructors InPair.
 
-(* * * * * BUNDLE DEFINITION * * * * *)
-Inductive ValidEdges (N: NodeSet) (E: EdgeSet) : Prop :=
-| validedges :
+
+Record Bundle : Type := Bundle_def
+{
+  Nodes : NodeSet;
+  Edges : EdgeSet;
+  FiniteNodes: FiniteSet Nodes;
+  FiniteEdges: FiniteSet Edges;
+  ValidEdges:
     (* N is the set of nodes incident with any edge in E *)
-    (and (forall x, InPair E x -> In Node N x)
+    (and (forall x, InPair Edges x -> In Node Nodes x)
     (* edges and the SSEdge property are equivalent *)
-         (forall x y, In Edge E (x,y) <-> x =-> y))
-    -> ValidEdges N E.
-(* TODO justification *)
+    (forall x y, In Edge Edges (x,y) <-> x =-> y));
+  ExistsUniqueTx:   
+    (forall z m, In Node Nodes z ->
+                 smsg(z) = (- m) -> 
+                 (* there exists a transmitter *)
+                 (exists x, (smsg(x) = (+ m)
+                             /\ x --> z
+                             /\ In Edge Edges (x,z)))
+                 (* a transmitter is unique *)
+                 /\ (forall x y, x --> z ->
+                                 y --> z ->
+                                 x = y));
+  Acyclic: forall x, ~ x << x
+}.
 
-Definition ExistsUniqueTx (N:NodeSet) (E:EdgeSet) : Prop :=
-  (forall z m, In Node N z ->
-              smsg(z) = (- m) -> 
-              (* there exists a transmitter *)
-              (exists x, (smsg(x) = (+ m)
-                          /\ x --> z
-                          /\ In Edge E (x,z)))
-              (* a transmitter is unique *)
-              /\ (forall x y, x --> z ->
-                              y --> z ->
-                              x = y)).
-(* TODO justification *)
+Definition StrandIn (s:Strand) (B:Bundle) :=
+  forall n, (strand n) = s -> In Node (Nodes B) n.
 
-Definition Acyclic (N:NodeSet) (E:EdgeSet) : Prop :=
-forall x, ~ x << x.
-(* TODO justification *)
-
-Definition Bundle (N:NodeSet) (E:EdgeSet) : Prop :=
-             Finite Node N /\
-             Finite Edge E /\
-             ValidEdges N E /\
-             ExistsUniqueTx N E /\
-             Acyclic N E.
-
-Lemma bundle_ssedge_inclusion : forall N E n m,
-Bundle N E ->
+Lemma bundle_ssedge_inclusion : forall (B: Bundle) (n m: Node),
 n =-> m ->
-(In Node N n -> In Node N m) /\ (In Node N m -> In Node N n).
+(In Node (Nodes B) n <-> In Node (Nodes B) m).
 Proof.
-  intros N E n m B ssedge. split; intros Hin.
-  destruct B as [finN [finE [valE [uniqtx acyc]]]].
+  intros B n m ssedge. split; intros Hin.
+  destruct B as [N E finN finE valE uniqtx acyc]; simpl in *.
   apply valE in ssedge. apply valE. constructor 2.
   exists n. exact ssedge.
-  destruct B as [finN [finE [valE [uniqtx acyc]]]].
+  destruct B as [N E finN finE valE uniqtx acyc].
   apply valE in ssedge. apply valE. constructor 1.
   exists m. exact ssedge.
 Qed.
 
-Definition bundle_set (s: ListSet.set Node) (N:NodeSet) : Prop :=
+Definition node_set_Ensemble_equiv (s: ListSet.set Node) (N:NodeSet) : Prop :=
 forall x, ListSet.set_In x s <-> In Node N x.
              
 Lemma sspath_imp_ssedge_l : forall x y,
@@ -667,14 +658,13 @@ Proof.
   exact IHsspath2.
 Qed.  
 
-Lemma restricted_to_set : forall N E,
-Bundle N E ->
+Lemma restricted_to_set : forall (B:Bundle),
 exists s, is_restricted SSEdge s /\
-forall x, ListSet.set_In x s <-> In Node N x.
+forall x, ListSet.set_In x s <-> In Node (Nodes B) x.
 Proof.
-  intros N E B.
-  destruct B as [finN [finE [valE [uniqtx acyc]]]].
-  destruct valE as [[EimpInN EimpSSEdge]].
+  intros B.
+  destruct B as [N E finN finE valE uniqtx acyc]; simpl in *.
+  destruct valE as [EimpInN EimpSSEdge].
   destruct (ensemble_imp_set Node eq_node_dec N finN) 
     as [s [inAll [nodup [n [slen scard]]]]].
   exists s.
@@ -688,14 +678,13 @@ Proof.
   exact inAll.
 Qed.
 
-Lemma sspath_dec : forall N E s,
-Bundle N E ->
-bundle_set s N ->
+Lemma sspath_dec : forall (B: Bundle) (s: ListSet.set Node),
+node_set_Ensemble_equiv s (Nodes B) ->
 is_restricted SSEdge s ->
 forall x y, {x << y} + {~x << y}.
 Proof.
-  intros N E s B bset restrict.
-  destruct B as [finN [finE [valE [uniqtx acyc]]]].
+  intros B s bset restrict.
+  destruct B as [N E finN finE valE uniqtx acyc]; simpl in *.
   intros x y.
   remember (restricted_dec_clos_trans_dec 
               eq_node_dec 
@@ -704,7 +693,7 @@ Proof.
   apply alldec.
 Qed.
 
-Lemma neq_sspatheq_imp_sspath : forall x y,
+Lemma neq_sspatheq_imp_sspath : forall (x y: Node),
 x <> y ->
 x <<* y ->
 x << y.
@@ -724,7 +713,7 @@ Proof.
         apply IHpatheqxy2. exact neqyz.
 Qed.      
 
-Lemma sspatheq_trans_cycle : forall x y,
+Lemma sspatheq_trans_cycle : forall (x y: Node),
 x <> y ->
 x <<* y ->
 y <<* x ->
@@ -740,11 +729,11 @@ Proof.
     exact patheqyx.
 Qed.
 
-Lemma bunble_partial_order : forall N E,
-Bundle N E ->
+(* Lemma 2.7a (partial order)  *)
+Lemma bunble_partial_order : forall (B:Bundle),
 Order Node SSPathEq.
 Proof.
-  intros N E B.
+  intros B.
   split.
   Case "Reflexivity".
     intros x. apply rt_refl. 
@@ -753,7 +742,7 @@ Proof.
     eapply rt_trans. exact xy. exact yz.
   Case "AntiSymmetry".
     intros x y xy yz.
-    destruct B as [finN [finE [valE [uniqtx acyc]]]].
+    destruct B as [N E finN finE valE uniqtx acyc]; simpl in *.
     destruct (eq_node_dec x y) as [xyeq | xyneq].
     SCase "x = y". exact xyeq.
     SCase "x <> y". 
@@ -762,12 +751,11 @@ Proof.
         exact xy. exact yz. apply acyc in contraxx. inversion contraxx.
 Qed.
 
-Lemma sspath_strict_order : forall N E,
-Bundle N E ->
+Lemma sspath_strict_order : forall (B: Bundle),
 StrictOrder Node SSPath.
 Proof.
-  intros N E B.
-  destruct B as [finN [finE [valE [uniqtx acyc]]]].
+  intros B.
+  destruct B as [N E finN finE valE uniqtx acyc]; simpl in *.
   split.
   Case "Irreflexivity".
     intros x. apply acyc.
@@ -780,29 +768,29 @@ In Node N n /\
 (forall x, In Node N x ->
            ~ x << n).
 
-Lemma bundle_subset_minimal : forall N E N',
-Bundle N E ->
-Included Node N' N ->
+(* Lemma 2.7b (non-empty subsets contain minimal members) *)
+Lemma bundle_subset_minimal : forall B N',
+Included Node N' (Nodes B) ->
 N' <> Empty_set Node ->
 exists min, set_minimal N' min.
 Proof.
-  intros N E N' B incl nempty.
-  assert (Bundle N E) as bundle. exact B.
-  destruct B as [finN [finE [valE [uniqtx acyc]]]].
+  intros B N' incl nempty.
+  remember B as bundle.
+  destruct bundle as [N E finN finE valE uniqtx acyc]; simpl in *.
   assert (Finite Node N') as finN'. eapply Finite_downward_closed.
     exact finN. exact incl.
   destruct (finite_cardinal Node N' finN') as [n card].
   destruct n. inversion card. rewrite H in nempty.
   assert False as F. apply nempty. reflexivity. inversion F.
-  destruct (restricted_to_set N E bundle) as [s [restricted setequiv]].
+  destruct (restricted_to_set B) as [s [restricted setequiv]].
   assert (forall x y, {x << y} + {~ x << y}) as rdec.
-  apply (sspath_dec N E s bundle). exact setequiv. exact restricted.  
+  apply (sspath_dec B s). exact setequiv. exact restricted.  
   destruct (minimal_finite_ensemble_mem 
               Node 
               eq_node_dec 
               SSPath 
               rdec
-              (sspath_strict_order N E bundle) 
+              (sspath_strict_order B) 
               N' 
               n 
               card) as [min [minIn nolt]].
@@ -810,43 +798,43 @@ Proof.
 Qed.
 
 (* Lemma 2.8 - set minimal is tx *)
-Lemma minimal_is_tx : forall N E N',
-Bundle N E ->
-Included Node N' N ->
-(forall m m', (In Node N m 
-               /\ In Node N m'
+Lemma minimal_is_tx : forall B N',
+Included Node N' (Nodes B) ->
+(forall m m' : Node, (In Node (Nodes B) m 
+               /\ In Node (Nodes B) m'
                /\ msg(m) = msg(m')) -> (* ADDED in N conditions *)
                (In Node N' m <-> In Node N' m')) ->
 forall n, set_minimal N' n ->
 is_tx n.
 Proof.
-  intros N E N' bundle sub incl n setmin.
-  remember bundle as B.
-  destruct bundle as [finN [finE [valE [uniqtx acyc]]]].
-  remember (Node_smsg n) as nsmsg. symmetry in Heqnsmsg.
+  intros B N' sub incl n setmin.
+  remember B as bundle.
+  destruct bundle as [N E finN finE valE uniqtx acyc]; simpl in *.
+  assert ((Nodes B) = N) as NB. subst B. simpl. reflexivity.
+  remember (smsg n) as nsmsg. symmetry in Heqnsmsg.
   destruct nsmsg.
   exists m. exact Heqnsmsg.
   unfold ExistsUniqueTx in uniqtx.
   assert (In Node N n) as nIn. destruct setmin; auto.
   destruct (uniqtx n m nIn Heqnsmsg) as [[ntx [ntxsmsg [commn inE]]] uniq].
   assert False as F. destruct setmin. apply (H0 ntx). eapply incl.
-    split. eapply bundle_ssedge_inclusion. exact B. constructor. exact commn.
-    exact nIn. split. exact nIn.
-    apply node_smsg_msg_rx in Heqnsmsg. apply node_smsg_msg_tx in ntxsmsg.
-    rewrite ntxsmsg. symmetry. exact Heqnsmsg. exact H.
-    constructor. constructor. exact commn.
+    split. rewrite <- NB. eapply bundle_ssedge_inclusion. 
+    constructor. exact commn. rewrite NB. exact nIn. 
+    split. exact nIn. apply node_smsg_msg_tx in ntxsmsg. 
+    apply node_smsg_msg_rx in Heqnsmsg. rewrite Heqnsmsg. exact ntxsmsg. 
+    exact H. constructor. constructor. exact commn.
   inversion F.
 Qed.
 
 Definition OccursIn (t:Msg) (n:Node) : Prop :=
-Subterm t msg(n).
+ t <st msg(n).
  (* [REF 1] Definition 2.3.5 pg 6
    "An unsigned term t occurs in n iff t is a subterm of the term of n" *)
 
 (* As close to paper def as possible *)
 Definition EntryPoint (n:Node) (I: Ensemble Msg) : Prop :=
 (exists t, In Msg I t /\ smsg(n) = (+ t))
-/\ forall n', n' << n -> ~ In Msg I msg(n').
+/\ forall n', n' << n -> ~ In Msg I (msg(n')).
  (* [REF 1] Definition 2.3.6 pg 6
    "Suppose I is a set of unsigned terms. The node n is an entrypoint for I
     iff term(n) = +t for some t in I, and forall n' s.t. n' =>+ n, term(n')
@@ -854,7 +842,7 @@ Definition EntryPoint (n:Node) (I: Ensemble Msg) : Prop :=
 
 (* As close to paper def as possible *)
 Definition Origin_with_Ex_Set (t:Msg) (n:Node) : Prop :=
-exists I, (forall t', Subterm t t' <-> In Msg I t')
+exists I, (forall t', t <st t' <-> In Msg I t')
 /\ EntryPoint n I.
  (* [REF 1] Definition 2.3.7 pg 6
    "An unsigned term t originates on n iff n is an entry point
@@ -862,18 +850,18 @@ exists I, (forall t', Subterm t t' <-> In Msg I t')
 
 Definition Origin (t:Msg) (n:Node) : Prop :=
 is_tx n
-/\ Subterm t msg(n)
-/\ forall n', n' << n -> ~Subterm t msg(n').
+/\ t <st msg(n)
+/\ forall n', n' << n -> ~t <st msg(n').
 
 Lemma Origin_imp_strict_defs : forall I t n,
-(forall t', Subterm t t' <-> In Msg I t') ->
+(forall t', t <st t' <-> In Msg I t') ->
 Origin t n ->
 Origin_with_Ex_Set t n.
 Proof.
   intros I t n Iprop Orig.
   exists I. split. exact Iprop.
   destruct Orig as [ntx [nsub nosucc]].
-  split. exists (Node_msg n).
+  split. exists (msg n).
   split. apply Iprop in nsub. exact nsub.
   destruct ntx. erewrite node_smsg_msg_tx. exact H. exact H.
   intros n' succ contraIn.
@@ -887,37 +875,37 @@ exists n, Origin t n
    "An unsigned term t is uniquely originating iff t originates on
     a unique n." *)
 
-(* Lemma 2.9 *)
-Lemma min_origin : forall N E N' n t,
-Bundle N E ->
-(forall m, (In Node N m 
-           /\ Subterm t msg(m)) <-> 
+(* Lemma 2.9 originating occurrence at minimal element *)
+Lemma min_origin : forall B N' n t,
+(forall m, (In Node (Nodes B) m 
+           /\ Subterm t (msg(m))) <-> 
            In Node N' m) ->
 set_minimal N' n ->
 Origin t n.
 Proof.
-  intros N E N' n t bundle N'def nmin.
-  remember bundle as B.
-  destruct bundle as [finN [finE [valE [uniqtx acyc]]]].
+  intros B N' n t N'def nmin.
+  remember B as bundle.
+  destruct bundle as [N E finN finE valE uniqtx acyc]; simpl in *.
+  assert (N = Nodes B) as NB. subst B. simpl; reflexivity.
   assert (In Node N' n) as nIn. destruct nmin; auto.
-  assert (Subterm t (Node_msg n)) as tsubn.
+  assert (t <st (msg n)) as tsubn.
     apply (N'def n) in nIn. destruct nIn; auto.
   assert (is_tx n) as nistx.
     assert (Included Node N' N) as incl.
       intros x xIn. apply N'def in xIn. destruct xIn; auto.
-    apply (minimal_is_tx N E N' B incl).
+    rewrite NB in incl. apply (minimal_is_tx B N' incl).
     intros x y eqmsg.
     destruct eqmsg as [xIn [yIn eqmsg]].
     split; intros Hin.
     Case "m in -> m' in".
       apply N'def in Hin. destruct Hin as [xInN tsubx]. 
-      assert (Subterm t (Node_msg y)) as ysubt. rewrite <- eqmsg.
+      assert (Subterm t (msg y)) as ysubt. rewrite <- eqmsg.
         exact tsubx.
-      apply N'def. split. exact yIn. exact ysubt.
+      apply N'def. split. rewrite NB. exact yIn. exact ysubt.
     Case "m' in -> m in".
       apply N'def in Hin. destruct Hin as [yInN tsuby].
-      apply N'def. split. exact xIn. 
-      assert (Subterm t (Node_msg x)) as xsubt. rewrite eqmsg.
+      apply N'def. split. rewrite NB. exact xIn. 
+      assert (Subterm t (msg x)) as xsubt. rewrite eqmsg.
         exact tsuby.
       exact xsubt. 
     exact nmin.
@@ -926,7 +914,7 @@ Proof.
   intros n' succn' contrasub.
   assert (In Node N' n') as n'In.
     apply N'def. split.
-    destruct valE as [[pairImpN HInEedge]].
+    destruct valE as [pairImpN HInEedge].
     apply pairImpN. left.
     destruct (sspath_imp_ssedge_l n' n succn') as [x n'edge].
     exists x. apply HInEedge. exact n'edge. exact contrasub.
@@ -936,7 +924,7 @@ Qed.
 
 (* Axiom 1 -- provable in this context *)
 Theorem free_encryption : forall m1 m2 k1 k2,
-[m1]^(k1) = [m2]^(k2) -> m1 = m2 /\ k1 = k2.
+[m1]^|k1| = [m2]^|k2| -> m1 = m2 /\ k1 = k2.
 Proof.
   intros m m' k k' encreq.
   inversion encreq. split; auto. 
@@ -953,11 +941,11 @@ Qed.
 (* Axiom 2 -- provable in this context *)
 Theorem free_term_algebra : forall m m' n n' k k' t,
 (m * n = m' * n' -> m = m' /\ n = n')
-/\ m * n <> [m']^(k)
+/\ m * n <> [m']^|k|
 /\ (#k) <> m * n
 /\ (!t) <> m * n
-/\ (#k) <> [m]^(k')
-/\ (!t) <> [m]^(k).
+/\ (#k) <> [m]^|k'|
+/\ (!t) <> [m]^|k|.
 Proof.
   intros m m' n n' k k' t;
   split. intros eq. inversion eq; auto. 
@@ -968,22 +956,21 @@ Proof.
   intros F. inversion F.
 Qed.
 
-Fixpoint msg_width (m:Msg) : nat :=
+Fixpoint width (m:Msg) : nat :=
 match m with
 | msg_text _ => 1
 | msg_key _ => 1
 | msg_encr _  _ => 1
-| msg_join x y => msg_width x + msg_width y
+| msg_join x y => width x + width y
 end.
 (* [REF 1] Definition 2.10 *)
 
-Notation "width( m )" := (msg_width m).
 
 (* Proposition 2.12 *)
 Lemma encr_subterm_imp : forall k k' h h',
 k <> k' ->
-Subterm [h']^(k') [h]^(k) ->
-Subterm [h']^(k') h.
+[h']^|k'| <st [h]^|k| ->
+[h']^|k'| <st h.
 Proof.
   intros k k' h h' kneq st.
   inversion st; subst.
@@ -991,43 +978,134 @@ Proof.
   exact H1.
 Qed.
 
-Definition PrincipalAlignment := Strand -> Prop.
-Variable Regular : PrincipalAlignment.
 Variable Inv : relation Key.
+(* Used to indicate two keys are cryptographic
+   inverses of eachother. *)
 
-Inductive Penetrator : KeySet -> PrincipalAlignment :=
-| pM : forall K s g, 
-        ~Regular s ->
-        s = [(+g)] -> 
-        Penetrator K s
-| pF : forall K s g, 
-        ~Regular s ->
-        s = [(-g)] -> 
-        Penetrator K s
-| pT : forall K s g, 
-        ~Regular s ->
-        s = [(-g), (+g), (+g)] ->
-        Penetrator K s
-| pC : forall K s g h, 
-        ~Regular s ->
-        s = [(-g), (-h), (+g*h)] ->
-        Penetrator K s
-| pS : forall K s g h, 
-        ~Regular s ->
-        s = [(-g*h), (+g), (+h)] ->
-        Penetrator K s
-| pK : forall K s k, 
-        ~Regular s ->
-        In Key K k ->
-        s = [(+ (#k))] ->
-        Penetrator K s
-| pE : forall K s h k,
-        ~Regular s ->
-        s = [(- (#k)), (-h), (+ [h]^(k))] ->
-        Penetrator K s
-| pD : forall K s h k k',
-        ~Regular s ->
-        Inv k' k ->
-        s = [(- (#k')), (- [h]^(k)), (+h)] ->
-        Penetrator K s.
+Variable Kp : Ensemble Key.
+(* Keys which are assumed to be initially known
+   by the penetrator. *)
+
+Variable UnkTp : Ensemble Text.
+(* Texts explicitly unknown to penetrators.
+   (this should allow something like a secret nonce to
+   not merely be "guessed" by a penetrator transmitting a
+   msg)  *)
+
+Variable Regular : Strand -> Prop.
+
+Inductive Penetrator : Strand -> Prop :=
+| P_M : forall s t, 
+          ~Regular s ->
+          ~ In Text UnkTp t ->
+          s = [(+(!t))] -> 
+          Penetrator s
+| P_F : forall s g, 
+          ~Regular s ->
+          s = [(-g)] -> 
+          Penetrator s
+| P_T : forall s g,
+          ~Regular s ->
+          s = [(-g), (+g), (+g)] ->
+          Penetrator s
+| P_C : forall s g h,
+          ~Regular s ->
+          s = [(-g), (-h), (+g*h)] ->
+          Penetrator s
+| P_S : forall s g h,
+          ~Regular s ->
+          s = [(-g*h), (+g), (+h)] ->
+          Penetrator s
+| P_K : forall s k,
+          ~Regular s ->
+          In Key Kp k ->
+          s = [(+ (#k))] ->
+          Penetrator s
+| P_E : forall s h k,
+          ~Regular s ->
+          s = [(- (#k)), (-h), (+ [h]^|k|)] ->
+          Penetrator s
+| P_D : forall s h k k',
+          ~Regular s ->
+          Inv k' k ->
+          s = [(- (#k')), (- [h]^|k|), (+h)] ->
+          Penetrator s.
+(* [REF 1] Definition 3.1
+    The set of atomic actions/traces a penetrator
+    may perform. *)
+
+Definition PenetratorNode (n:Node) : Prop :=
+Penetrator (strand(n)).
+
+Definition RegularNode (n:Node) : Prop :=
+Regular (strand(n)).
+
+Lemma st_dec : forall a b,
+{a <st b} + {~ a <st b}.
+Proof.
+  intros a b.
+  induction b.
+  Case "b = txt".
+    destruct a.
+    SCase "a = txt".
+      destruct (eq_text_dec t t0).
+        subst t. left. auto.
+        right. intros contra. inversion contra. 
+        symmetry in H1. contradiction.
+    SCase "a = key". right. intros contra. inversion contra.
+    SCase "a = join". right. intros contra. inversion contra.
+    SCase "a = encr". right. intros contra. inversion contra.
+  Case "b = key".
+    destruct a.
+    SCase "a = txt". right. intros contra. inversion contra.
+    SCase "a = key".
+      destruct (eq_key_dec k k0).
+        subst k. left. auto.
+        right. intros contra. inversion contra. 
+        symmetry in H1. contradiction.
+    SCase "a = join". right. intros contra. inversion contra.
+    SCase "a = encr". right. intros contra. inversion contra.
+  Case "b = join".
+    destruct IHb1.
+    SCase "a <st b1". left. apply st_join_l. exact s.
+    SCase "~a <st b1". 
+      destruct IHb2.
+      SSCase "a <st b2". left. apply st_join_r. exact s.
+      SSCase "~a <st b2". 
+        destruct (eq_msg_dec a (b1 * b2)).
+        SSSCase "a = b1 * b2".
+          subst a. left. constructor.
+        SSSCase "a <> b1 * b2".
+          right. intros contra. inversion contra; subst; try(contradiction).
+          apply n1. reflexivity.
+  Case "b = encr".
+    destruct IHb.
+      left. apply st_encr. exact s.
+      destruct (eq_msg_dec a ([b]^|k|)). subst.
+      left. constructor.
+      right. intros contra. inversion contra. subst.
+      apply n0. reflexivity.
+      contradiction.
+Qed.
+
+(* Proposition 3.3 
+   "Let C be a bundle, and let k be a Key s.t. ~ k in Kp,
+   If k never originates on a regular node, then K is not
+   a subterm of term(n) for any node n in C. In particular,
+   for any penetrator node p in C, k is not a subterm
+   of the term of p." *)
+Theorem non_origin_imp_non_subterm : forall B k,
+~ In Key Kp k ->
+(forall n, Origin (#k) n -> ~ RegularNode n) ->
+(forall n, In Node (Nodes B) n -> ~ (#k) <st msg(n)).
+Proof.
+  intros B k notInKp noOrigin n nInN st.
+  eapply noOrigin.
+  unfold Origin.
+
+Theorem non_subterm_incl_penetrators : forall B k,
+(forall n, In Node (Nodes B) n -> ~ (#k) <st msg(n)) ->
+(forall p, In Node (Nodes B) p -> 
+              PenetratorNode p ->
+              ~ (#k) <st msg(p)).
 
